Generalize Equiv_ctx to source programs that may not be safe, by proving that Compositional CompCert implies behavior refinement:   If linked C[prog2] diverges, then C[prog1] diverges or goes wrong.   If linked C[prog2] terminates, then C[prog1] terminates or goes wrong. Proof currently uses excluded middle but this can be fixed. This notion of program refinement is a preorder (reflexive and transitive).

linking/context_equiv.v
@@ -119,6 +119,51 @@ case: (H2 C main args m Inv c2 Init2 Hsafe2)=> c3 []Init3 Hsafe3 Hterm23.
 by exists c3; split=> //; rewrite Hterm12 Hterm23.
 Qed.
 
+Definition Prog_refines (ge : ge_ty) (N : pos) plt (p1 p2 : Prog.t N) :=
+  forall C : Ctx.t ge,
+  forall (main : val) (args : list val) m,
+  cc_init_inv (Mem.flat_inj (Mem.nextblock m)) ge args m ge args m -> 
+  forall c1, initial_core (link_ctx C p1 plt) ge main args = Some c1 -> 
+  exists c2,
+  [/\ initial_core (link_ctx C p2 plt) ge main args = Some c2
+    & forall tbeh, has_behavior (link_ctx C p2 plt) ge c2 m tbeh -> 
+      exists beh, 
+      [/\ has_behavior (link_ctx C p1 plt) ge c1 m beh
+        & behavior_refines tbeh beh]].
+
+Lemma behavior_refines_refl beh : behavior_refines beh beh.
+Proof. by case: beh; constructor. Qed.
+
+Lemma behavior_refines_trans beh1 beh2 beh3 : 
+  behavior_refines beh1 beh2 -> 
+  behavior_refines beh2 beh3 -> 
+  behavior_refines beh1 beh3.
+Proof.
+inversion 1; subst; auto. 
+inversion 1; subst; auto.
+Qed.
+
+Lemma Prog_refines_refl ge N plt (p : Prog.t N) : Prog_refines ge plt p p.
+Proof.
+move=> C main args m Inv c1 Init1; exists c1; split=> //.
+move=> tbeh Has1; exists tbeh; split=> //; last by apply: behavior_refines_refl.
+Qed.
+
+Lemma Prog_refines_trans ge N plt (p1 p2 p3 : Prog.t N) : 
+  Prog_refines ge plt p1 p2 -> 
+  Prog_refines ge plt p2 p3 -> 
+  Prog_refines ge plt p1 p3.
+Proof.
+move=> H1 H2 C main args m Inv c1 Init1.
+case: (H1 C main args m Inv c1 Init1)=> c2 []Init2 X2.
+case: (H2 C main args m Inv c2 Init2)=> c3 []Init3 X3.
+exists c3; split=> // beh3 Has3. 
+case: (X3 beh3 Has3)=> beh2 []Has2 R2.
+case: (X2 beh2 Has2)=> beh1 []Has1 R1.
+exists beh1; split=> //.
+by apply: (behavior_refines_trans R2 R1).
+Qed.
+
 (** Prove that Simulation implies Equiv_ctx *)
 
 Module ContextEquiv (LS : LINKING_SIMULATION). 
@@ -228,6 +273,60 @@ Qed.
 End ContextEquiv.
 
 End ContextEquiv2.
+
+(** Prove that Simulation implies behavior refinement *)
+
+Module ProgRefines (LS : LINKING_SIMULATION). 
+                                                                       
+Import LS.                                                             
+                                                                       
+Section ProgRefines.
+
+Variable N : pos.
+Variable pS pT : Prog.t N.
+Variable rclosed_S : forall ix : 'I_N, RCSem.t (Prog.sems pS ix).(sem) (Prog.sems pS ix).(ge).
+Variable valid_T : forall ix : 'I_N, Nuke_sem.t (Prog.sems pT ix).(sem).
+Variable targets_det : forall ix : 'I_N, corestep_fun (Prog.sems pT ix).(sem).
+Variable plt : ident -> option 'I_N.
+Variable sims : 
+  forall ix : 'I_N,                                          
+  let s := Prog.sems pS ix in                                              
+  let t := Prog.sems pT ix in                                              
+  SM_simulation_inject s.(sem) t.(sem) s.(ge) t.(ge).
+Variable ge_top : ge_ty.                                                     
+Variable domeq_S : forall ix : 'I_N, genvs_domain_eq ge_top (Prog.sems pS ix).(ge).
+Variable domeq_T : forall ix : 'I_N, genvs_domain_eq ge_top (Prog.sems pT ix).(ge). 
+Variable find_symbol_ST : 
+  forall (ix : 'I_N) id bf, 
+  Genv.find_symbol (ge (Prog.sems pS ix)) id = Some bf -> 
+  Genv.find_symbol (ge (Prog.sems pT ix)) id = Some bf.
+
+Lemma refines (EM : ClassicalFacts.excluded_middle) : Prog_refines ge_top plt pS pT.
+Proof.
+rewrite /Equiv_ctx=> C main args m Init c1 Init1.
+have sim: CompCert_wholeprog_sim (link_ctx C pS plt) (link_ctx C pT plt) ge_top ge_top main.
+{ apply: link=> ix; rewrite /Prog.sems/apply_ctx/extend_sems. 
+  by move=> ??; case e: (lt_dec ix N)=> [pf|pf] //; apply find_symbol_ST.
+  by case e: (lt_dec ix N)=> [pf|pf] //; apply: (Ctx.rclosed_C C).
+  by case e: (lt_dec ix N)=> [pf|pf] //; apply: (Ctx.valid_C C).
+  by case e: (lt_dec ix N)=> [pf|pf] //; apply: (Ctx.sim_C C).
+  by case e: (lt_dec ix N)=> [pf|pf] //; apply: (Ctx.domeq_C C).
+  by case e: (lt_dec ix N)=> [pf|pf] //; apply: (Ctx.domeq_C C). }
+have target_det: corestep_fun (link_ctx C pT plt). 
+{ apply: linking_det=> ix; rewrite /Prog.sems/apply_ctx/extend_sems.
+  by case e: (lt_dec ix N)=> [pf|pf] //; apply Ctx.det_C. }
+eapply @core_initial 
+  with (Sem1 := link_ctx C pS plt) (Sem2 := link_ctx C pT plt) 
+       (ge1 := ge_top) (ge2 := ge_top) (halt_inv := cc_halt_inv)
+       (j := Mem.flat_inj (Mem.nextblock m)) (main := main) (m1 := m) (m2 := m) (w := sim)
+  in Init1; eauto.
+case: Init1=> mu []cd []c2 []_ []Init2' Hmatch.
+by exists c2; split=> //; first by move=> tbeh; eapply behavior_refinment; eauto.
+Qed.
+
+End ProgRefines.
+
+End ProgRefines.
 
 
 
